Weidenbach_Book/IsaSAT/IsaSAT_Restart_Heuristics_LLVM.thy
@@ -1,6 +1,6 @@
 theory IsaSAT_Restart_Heuristics_LLVM
   imports IsaSAT_Restart_Heuristics IsaSAT_Setup_LLVM
-     IsaSAT_VMTF_LLVM IsaSAT_Rephase_LLVM
+     IsaSAT_VMTF_State_LLVM IsaSAT_Rephase_LLVM
      IsaSAT_Arena_Sorting_LLVM
 begin
 
