Weidenbach_Book/IsaSAT/IsaSAT_VMTF_State_LLVM.thy
@@ -1,0 +1,21 @@
+theory IsaSAT_VMTF_State_LLVM
+  imports IsaSAT_VMTF_LLVM IsaSAT_Setup_LLVM
+begin
+
+sepref_def find_decomp_wl_imp'_fast_code
+  is \<open>uncurry find_decomp_wl_st_int\<close>
+  :: \<open>uint32_nat_assn\<^sup>k *\<^sub>a isasat_bounded_assn\<^sup>d  \<rightarrow>\<^sub>a
+        isasat_bounded_assn\<close>
+  unfolding find_decomp_wl_st_int_def PR_CONST_def isasat_bounded_assn_def
+  supply [[goals_limit = 1]]
+  unfolding fold_tuple_optimizations
+  by sepref
+
+experiment begin
+
+export_llvm
+  find_decomp_wl_imp'_fast_code
+
+end
+
+end
